\documentclass[12pt]{article}
\usepackage{amsmath , amssymb}
\usepackage{graphicx}
\usepackage{float}
\usepackage{pgfplots}
\pgfplotsset{compat=1.18}
\newcommand{\tabref}[1]{Table~\ref{#1}}
\newcommand{\figref}[1]{Figure~\ref{#1}}
\providecommand{\abs}[1]{\left\vert#1\right\vert}

\begin{document}

\title{Discrete Assignment}
\author{Mohana Eppala\\ EE23BTECH11018}
\maketitle

\section*{Problem Statement}
Find the value of $n$ so that $\frac{a^{n+1} + b^{n+1}}{a^{n}+b^{n}}$ may be the geometric mean between $a$ and $b$.
\section{Solution}

\begin{table}[H]
\input{./tables/tab2.tex}
\end{table}

Consider a GP as in \tabref{tab:1},
\begin{align}
	\therefore \frac{a^{n+1} + b^{n+1}}{a^{n}+b^{n}} &= x(1) \\
	\implies a^{n+1} + b^{n+1} &= a^{n+\frac{1}{2}}b^{\frac{1}{2}} + a^{\frac{1}{2}}b^{n+\frac{1}{2}} \\ 
\implies a^{n+1} - a^{n+\frac{1}{2}}b^{\frac{1}{2}} &=  a^{\frac{1}{2}}b^{n+\frac{1}{2}} - b^{n+1} \\ 
\implies a^{n+\frac{1}{2}}(a^{\frac{1}{2}} - b^{\frac{1}{2}}) &= b^{n+\frac{1}{2}}(a^{\frac{1}{2}} - b^{\frac{1}{2}}) \\     
\implies a^{n+\frac{1}{2}} &= b^{n+\frac{1}{2}} \\ 
\implies (\frac{a}{b})^{n+\frac{1}{2}} &= (\frac{a}{b})^{0} \\
\implies n + \frac{1}{2} &= 0 \\
\implies n &= -\frac{1}{2}
\end{align}
From \tabref{tab:1},
\begin{align}
	X(z) &= \sum_{k=-\infty}^{\infty} (ar^{k})u(k) \\
	&= a(\frac{1}{1-r})(\frac{1}{1-z^{-1}}) \\
	&= a(\frac{1}{1-\sqrt(\frac{b}{a})})(\frac{1}{1-z^{-1}})
\end{align}
\end{document}
